# 1 Vibration ODEs

## 1.1 Finite Difference Discretization

### 1.1.1 A Basic Model for Vibrations

Consider the vibrating mechanical system
$$u''+\omega^2 u=0, \quad u(0)=I, \quad u'(0)=0, \quad t \in(0, T] \quad \quad \quad (1.1)$$
with constant amplitude $I$ and angular frequency $\omega$. The corresponsing period is $P=2\pi/\omega$, and the corresponding frequency is $f=\omega/(2\pi)$. In this system, $u(t)$ represents displacement, $u'(t)$ velocity, and $u''(t)$ acceleration. The exact solution of $(1.1)$ is $u(t)=I \cos (\omega t)$.

### 1.1.2 A Centered Finite Difference Scheme
Four steps are to follow to formulate a finite difference method for the problem $(1.1)$.

**Step 1: Discretizing the domain**

The domain is discretized by introducing a uniformly partitioned time mesh. The points in the mesh are $t_n=n \Delta t, n=0,1, \ldots ,N_t$, where $\Delta t=T/N_t$ is the constant length of the time steps. A mesh function $u^n$ for $n=0,1, \ldots, N_t$ is introduced to approximate the exact solution $u(t_n)$ at the mesh points: 
$$u(t_n) \sim u^n. \quad \quad \quad (1.2)$$
The mesh function $u^n$ will be computed from algebraic equations derived from the differential equation problem. 

**Step 2: Fulfilling the equation at discrete time points**

The ODE is to be satisfied at each mesh point, then the solutions must be found for
$$u''(t_n)+\omega^2 u(t_n)=0, \quad n=1, \ldots, N_t. \quad \quad \quad (1.3)$$

**Step 3: Replacing derivatives with finite differences**

By Taylor expansion, 
$$u(t+\Delta t)=u(t)+u'(t) \Delta +\frac{1}{2} u''(t)(\Delta t)^2+\frac{1}{6} u'''(t)(\Delta t)^3+O((\Delta t)^4),$$
$$u(t-\Delta t)=u(t)-u'(t) \Delta +\frac{1}{2} u''(t)(\Delta t)^2-\frac{1}{6} u'''(t)(\Delta t)^3+O((\Delta t)^4).$$
Adding these two expansions and solving for $u''(t)$, we have
$$u''(t)=\frac{u(t+\Delta t)-2 u(t)+u(t-\Delta t)}{(\Delta t)^2}+O((\Delta t)^2).$$
Replacing $t$ by $t_n=n \Delta t$ and using $(1.2)$ yields the common second-order accurate centered approximation to the second-order derivative
$$u''(t_n) \sim  \frac{u^{n+1}-2 u^n+u^{n-1}}{\Delta t^2} \quad \quad \quad (1.4)$$
Inserting $(1.2)$ and $(1.4)$ into $(1.3)$, we have
$$\frac{u^{n+1}-2 u^n+u^{n-1}}{\Delta t^2}+\omega^2 u^n=0, \quad n=1, \ldots, N_t. \quad \quad \quad (1.5)$$
